Repair some of the compiler proofs
They were broken by the changes in the semantics, especially moving the
evalProps to semanticPrimitivesProps and evaluateProps, to following the
naming scheme.

Also change the top-level semantics so that Failing programs can't also
terminate usually with a final FFI event.

semantics/proofs/semanticsPropsScript.sml
@@ -23,8 +23,8 @@ val semantics_prog_total = Q.store_thm("semantics_prog_total",
   Cases_on`∃k ffi r.
     evaluate_prog_with_clock s e k p = (ffi,r) ∧
     r ≠ Rerr (Rabort Rtype_error) ∧
-    (ffi.final_event = NONE ⇒ ∀a. r ≠ Rerr (Rabort a))`
-  >- metis_tac[semantics_prog_def] >> full_simp_tac(srw_ss())[] >>
+    (ffi.final_event = NONE ⇒ r ≠ Rerr (Rabort Rtimeout_error))`
+  >- metis_tac[semantics_prog_def,SND] >> full_simp_tac(srw_ss())[] >>
   qexists_tac`Diverge (build_lprefix_lub (IMAGE (λk. fromList (FST (evaluate_prog_with_clock s e k p)).io_events) UNIV))` >>
   simp[semantics_prog_def] >>
   conj_tac >- (
@@ -41,51 +41,46 @@ val with_clock_ffi = Q.prove(
   `(s with clock := x).ffi = s.ffi`,EVAL_TAC)
 
 val tac1 =
-    metis_tac[semanticPrimitivesTheory.result_11,
-              semanticPrimitivesTheory.error_result_11,
-              semanticPrimitivesTheory.abort_distinct,
-              PAIR_EQ,IS_SOME_EXISTS,NOT_SOME_NONE,SND,PAIR]
+    metis_tac[semanticPrimitivesTheory.result_11,evaluate_prog_ffi_mono_clock,
+              semanticPrimitivesTheory.error_result_11,option_nchotomy,LESS_EQ_CASES,
+              semanticPrimitivesTheory.abort_distinct,pair_CASES,FST,THE_DEF,
+              PAIR_EQ,IS_SOME_EXISTS,SOME_11,NOT_SOME_NONE,SND,PAIR,LESS_OR_EQ]
 
-              (*
 val semantics_prog_deterministic = Q.store_thm("semantics_prog_deterministic",
   `∀s e p b b'.
-    semantics_prog s e p b ∧ b ≠ Fail ∧
-    semantics_prog s e p b' ∧ b' ≠ Fail ⇒
+    semantics_prog s e p b ∧
+    semantics_prog s e p b' ⇒
     b = b'`,
-  ntac 3 gen_tac >> reverse Cases >> srw_tac[][semantics_prog_def]
-  >- (
-    Cases_on`b'`>>full_simp_tac(srw_ss())[semantics_prog_def]
-    >- tac1
-    >- (
-      fs [evaluate_prog_with_clock_def, evaluate_prog_def]
-      qmatch_assum_abbrev_tac`if X then Y else Z` >>
-      reverse(Cases_on`X`)>>full_simp_tac(srw_ss())[Abbr`Y`,Abbr`Z`] >- (
-        rpt var_eq_tac >> full_simp_tac(srw_ss())[] ) >>
-      Cases_on`∃a a'. r = Rerr (Rabort a) ∧ r' = Rerr (Rabort a')` >> full_simp_tac(srw_ss())[] >- (
-        metis_tac[LESS_EQ_CASES,
-                  evaluate_prog_ffi_mono_clock,
-                  FST,THE_DEF,IS_SOME_EXISTS,NOT_SOME_NONE,option_CASES] ) >>
-      Cases_on`r = Rerr (Rabort Rtimeout_error) ∨ r' = Rerr (Rabort Rtimeout_error)` >- (
-        metis_tac[prog_clocked_timeout_smaller,
-                  LESS_IMP_LESS_OR_EQ,
-                  evaluate_prog_ffi_mono_clock,
-                  FST,THE_DEF,IS_SOME_EXISTS,NOT_SOME_NONE,option_CASES] ) >>
-      imp_res_tac prog_clocked_min_counter >> full_simp_tac(srw_ss())[] >>
-      first_x_assum(mp_tac o MATCH_MP (REWRITE_RULE[GSYM AND_IMP_INTRO](GEN_ALL prog_clocked_zero_determ))) >>
-      disch_then(fn th => first_x_assum(mp_tac o MATCH_MP th)) >>
-      simp[semanticPrimitivesTheory.state_component_equality] >>
-      srw_tac[][] >> every_case_tac >> rev_full_simp_tac(srw_ss())[]))
-  >- (
-    Cases_on`b'`>>full_simp_tac(srw_ss())[semantics_prog_def]
-    >- metis_tac[unique_lprefix_lub] >>
-    tac1))
-    *)
+ rw []
+ >> Cases_on `b`
+ >> Cases_on `b'`
+ >> fs [semantics_prog_def]
+ >- metis_tac[unique_lprefix_lub]
+ >- tac1
+ >- tac1
+ >- tac1
+ >- (
+   fs [evaluate_prog_with_clock_def]
+   >> pairarg_tac
+   >> fs []
+   >> pairarg_tac
+   >> fs []
+   >> rpt var_eq_tac
+   >> pop_assum mp_tac
+   >> drule evaluate_prog_clock_determ
+   >> ntac 2 DISCH_TAC
+   >> first_x_assum drule
+   >> simp []
+   >> every_case_tac
+   >> fs [semanticPrimitivesTheory.state_component_equality]
+   >> tac1)
+ >- tac1
+ >- tac1
+ >- tac1);
 
-    (*
 val state_invariant_def = Define`
   state_invariant st ⇔
-  type_sound_invariants (NONE:(v,v)result option) (st.tdecs,st.tenv,st.sem_st,st.sem_env)`;
-  *)
+  ?ctMap tenvS. type_sound_invariant st.sem_st st.sem_env st.tdecs ctMap tenvS st.tenv`;
 
 val clock_lemmas = Q.prove(
   `((x with clock := c).clock = c) ∧
@@ -93,65 +88,19 @@ val clock_lemmas = Q.prove(
    (x with clock := x.clock = x)`,
   srw_tac[][semanticPrimitivesTheory.state_component_equality])
 
-  (*
-val prog_diverges_semantics_prog = Q.store_thm("prog_diverges_semantics_prog",
-  `prog_diverges st.sem_env st.sem_st prog ∧
-   no_dup_mods prog st.sem_st.defined_mods ∧
-   no_dup_top_types prog st.sem_st.defined_types ⇒
-   ¬semantics_prog st.sem_st st.sem_env prog Fail`,
-  strip_tac >>
-  (untyped_safety_prog
-   |> SPEC_ALL
-   |> EQ_IMP_RULE |> fst
-   |> CONTRAPOS
-   |> SIMP_RULE bool_ss []
-   |> imp_res_tac) >>
-  simp[semantics_prog_def,PULL_EXISTS] >>
-  srw_tac[][evaluate_prog_with_clock_def] >>
-  imp_res_tac functional_evaluate_prog >>
-  rev_full_simp_tac(srw_ss())[bigStepTheory.evaluate_whole_prog_def] >>
-  full_simp_tac(srw_ss())[prog_clocked_unclocked_equiv,FORALL_PROD] >>
-  imp_res_tac prog_clocked_min_counter >> full_simp_tac(srw_ss())[] >>
-  spose_not_then strip_assume_tac >>
-  Cases_on`envC`>>full_simp_tac(srw_ss())[] >>
-  metis_tac[clock_lemmas,
-            semanticPrimitivesTheory.result_11,
-            semanticPrimitivesTheory.error_result_11,
-            semanticPrimitivesTheory.abort_distinct])
-            *)
-
-            (*
 val semantics_deterministic = Q.store_thm("semantics_deterministic",
   `state_invariant st ⇒
    semantics st prelude inp = Execute bs
    ⇒ ∃b. bs = {b} ∧ b ≠ Fail`,
-  srw_tac[][semantics_def] >> every_case_tac >> full_simp_tac(srw_ss())[] >> srw_tac[][] >>
-  `∀b. semantics_prog st.sem_st st.sem_env (prelude ++ x) b ⇒ b ≠ Fail` by(
-    full_simp_tac(srw_ss())[can_type_prog_def,state_invariant_def] >>
-    Cases_on`prog_diverges st.sem_env st.sem_st (prelude ++ x)` >- (
-      imp_res_tac prog_diverges_semantics_prog >> metis_tac[] ) >>
-    full_simp_tac(srw_ss())[semantics_prog_def,evaluate_prog_with_clock_def,LET_THM] >>
-    CCONTR_TAC >> full_simp_tac(srw_ss())[] >>
-    first_assum(split_uncurry_arg_tac o rand o lhs o concl) >>
-    imp_res_tac functional_evaluate_prog >>
-    (whole_prog_type_soundness
-     |> REWRITE_RULE[GSYM AND_IMP_INTRO]
-     |> (fn th => first_x_assum(mp_tac o MATCH_MP th))) >>
-    PairCases_on`new_tenv`>>
-    disch_then(fn th => first_x_assum(mp_tac o MATCH_MP th)) >>
-    simp[PULL_EXISTS] >> full_simp_tac(srw_ss())[] >>
-    rev_full_simp_tac(srw_ss())[bigStepTheory.evaluate_whole_prog_def] >>
-    simp[prog_clocked_unclocked_equiv,PULL_EXISTS] >>
-    CCONTR_TAC >> full_simp_tac(srw_ss())[] >>
-    imp_res_tac prog_clocked_min_counter >> full_simp_tac(srw_ss())[] >>
-    metis_tac[prog_clocked_zero_determ,SND,PAIR_EQ,
-              semanticPrimitivesTheory.result_11,
-              semanticPrimitivesTheory.result_distinct,
-              semanticPrimitivesTheory.error_result_11,
-              semanticPrimitivesTheory.abort_distinct]) >>
-  simp[FUN_EQ_THM] >>
-  metis_tac[semantics_prog_total,semantics_prog_deterministic])
-  *)
+ rw [state_invariant_def, semantics_def]
+ >> every_case_tac
+ >> fs [can_type_prog_def]
+ >> rw []
+ >> qspecl_then [`st.sem_st`, `st.sem_env`, `prelude ++ x`] strip_assume_tac semantics_prog_total
+ >> imp_res_tac semantics_type_sound
+ >> qexists_tac `b`
+ >> rw [EXTENSION, IN_DEF]
+ >> metis_tac [semantics_prog_deterministic]);
 
 val extend_with_resource_limit_def = Define`
   extend_with_resource_limit behaviours =
