semantics/proofs/evaluatePropsScript.sml
@@ -1,5 +1,6 @@
 open preamble evaluateTheory;
 open terminationTheory
+open semanticPrimitivesTheory;
 open semanticPrimitivesPropsTheory;
 
 val _ = new_theory"evaluateProps"
@@ -264,7 +265,7 @@ val evaluate_decs_cons = Q.store_thm ("evaluate_decs_cons",
  >> simp []
  >> rename1 `evaluate_decs _ _ _ _ = (s',ctors,r)`
  >> Cases_on `r`
- >> simp [semanticPrimitivesTheory.combine_dec_result_def]);
+ >> simp [combine_dec_result_def]);
 
 val evaluate_tops_nil = Q.store_thm("evaluate_tops_nil[simp]",
   `∀(s:'ffi state) env. evaluate_tops s env [] = (s,([],[]),Rval ([],[]))`,
@@ -285,7 +286,7 @@ val evaluate_tops_cons = Q.store_thm ("evaluate_tops_cons",
  >> simp []
  >> rename1 `evaluate_tops _ _ _ = (s',ctors,r)`
  >> Cases_on `r`
- >> simp [semanticPrimitivesTheory.combine_mod_result_def]
+ >> simp [combine_mod_result_def]
  >> split_pair_case_tac
  >> simp []);
 
@@ -322,7 +323,7 @@ val evaluate_decs_add_to_clock = Q.store_thm("evaluate_decs_add_to_clock",
     >> Cases_on `r'`
     >> fs []
     >> Cases_on `e'`
-    >> fs [semanticPrimitivesTheory.combine_dec_result_def])
+    >> fs [combine_dec_result_def])
   >- (
     every_case_tac
     >> fs []
@@ -357,7 +358,7 @@ val evaluate_tops_add_to_clock = Q.store_thm("evaluate_tops_add_to_clock",
      >> simp []
      >> rw []
      >> Cases_on `r''`
-     >> fs [semanticPrimitivesTheory.combine_mod_result_def])
+     >> fs [combine_mod_result_def])
    >- (
      rw []
      >> fs []))
@@ -375,8 +376,88 @@ val evaluate_tops_add_to_clock = Q.store_thm("evaluate_tops_add_to_clock",
    >> fs []
    >> rw []));
 
-  val with_clock_ffi = Q.prove(
+val add_lemma = Q.prove (
+ `!(k:num) k'. ?extra. k = k' + extra ∨ k' = k + extra`,
+ intLib.ARITH_TAC);
+
+val with_clock_with_clock = Q.prove (
+`((s with clock := x) with clock := y) = s with clock := y`,
+ rw []);
+
+val with_clock_ffi = Q.prove(
   `(s with clock := k).ffi = s.ffi`,EVAL_TAC)
+
+val tac1 =
+  metis_tac[result_distinct,result_11,evaluate_tops_add_to_clock,
+            error_result_11,error_result_distinct,option_nchotomy,
+            abort_distinct,pair_CASES,FST,with_clock_ffi,
+            PAIR_EQ,IS_SOME_EXISTS,SOME_11,NOT_SOME_NONE,SND,PAIR, add_lemma,
+            state_component_equality, with_clock_with_clock]
+
+val evaluate_prog_clock_determ = Q.store_thm ("evaluate_prog_clock_determ",
+`!s e p s1 c1 r1 s2 c2 r2 k1 k2.
+  evaluate_prog (s with clock := k1) e p = (s1,c1,r1) ∧
+  evaluate_prog (s with clock := k2) e p = (s2,c2,r2)
+  ⇒
+  case (r1,r2) of
+  | (Rerr (Rabort Rtimeout_error), Rerr (Rabort Rtimeout_error)) =>
+    T
+  | (Rerr (Rabort Rtimeout_error), _) =>
+    k1 < k2
+  | (_, Rerr (Rabort Rtimeout_error)) =>
+    k2 < k1
+  | _ =>
+    s1.ffi = s2.ffi ∧ c1 = c2 ∧ r1 = r2`,
+ rw []
+ >> Cases_on `r2 = Rerr (Rabort Rtimeout_error)`
+ >> Cases_on `r1 = Rerr (Rabort Rtimeout_error)`
+ >> fs []
+ >> fs []
+ >> fs []
+ >> rw []
+ >- (
+   `k2 < k1` suffices_by (every_case_tac >> fs [])
+   >> CCONTR_TAC
+   >> fs [evaluate_prog_def]
+   >> every_case_tac
+   >> fs []
+   >> `?extra. k2 = k1 + extra` by intLib.ARITH_TAC
+   >> qpat_assum `evaluate_tops _ _ _ = _` mp_tac
+   >> drule evaluate_tops_add_to_clock
+   >> rw [])
+ >- (
+   `k1 < k2` suffices_by (every_case_tac >> fs [])
+   >> CCONTR_TAC
+   >> fs [evaluate_prog_def]
+   >> every_case_tac
+   >> fs []
+   >> `?extra. k1 = k2 + extra` by intLib.ARITH_TAC
+   >> drule evaluate_tops_add_to_clock
+   >> fs []
+   >> qexists_tac `extra`
+   >> simp [])
+ >- (
+   fs [evaluate_prog_def]
+   >> qpat_assum `(if _ then _ else _) = _` mp_tac
+   >> CASE_TAC
+   >> rw []
+   >> rw []
+   >> qspecl_then [`k1`, `k2`] strip_assume_tac add_lemma
+   >> var_eq_tac
+   >| [
+     drule evaluate_tops_add_to_clock
+       >> simp []
+       >> disch_then (qspec_then `extra` mp_tac)
+       >> rw [],
+     qpat_assum `evaluate_tops _ _ _ = _` mp_tac
+       >> drule evaluate_tops_add_to_clock
+       >> simp []
+       >> disch_then (qspec_then `extra` mp_tac)
+       >> rw []]
+   >> every_case_tac
+   >> fs []
+   >> rw []));
+
 val lemma = DECIDE``x ≠ 0n ⇒ x - 1 + y = x + y - 1``
 
 val evaluate_add_to_clock_io_events_mono = Q.store_thm("evaluate_add_to_clock_io_events_mono",
